L_4,0 = (x-2,5).x.(x-2,5).(x-5) / (-5+2,5).(-5).(-5-2,5).(-5-5) = (x^4 - 6,35x^2 -5x^3 - 31,52x) / 937,5

L_4,1 = (x-2,5).x.(x-2,5).(x-5) / (-5+2,5).(-5).(-5-2,5).(-5-5) = x^4 - 2,5x^3 - 25x^3 + 62,5x / 234,375

L_4,2 = (x + 5).(x+2,5).(x-2,5).(x-5) / (2,5).5.(-5).(-2,5) = (x^2 + 25).(x^2 + 6,25) / 156.25

L_4,3 = (x + 5).(x + 2,5).x.(x - 5) / (2,5 + 5).(2,5 + 2,5).2,5.(2,5 - 5) = (x^2 - 25).x.(x + 2,5) / âˆ’234,375

L_4,4 = (x + 5).(x + 2,5).x.(x - 2,5) / (5 + 5).(5 + 2,5).5.(5 - 2,5) = (x^2 + 5x).(x^2 - 6,25) / 937,5

f(x_0) = 1 / (1 + (-5)^2) = 1 / 1 + 25 = 1 / 26

f(x_1) = 1 / (1 + (-2,5)^2) = 1 / 1 + 6,25 = 1 / 7,25

f(x_2) = 1 / (1 + 0^2) = 1 / 1 + 0 = 1 / 1 = 1

f(x_3) = f(x_1)

f(x_4) = f(x_0)
